# 2019-11-15

1. Product decomposition
   Consider net
   ```
    E     B
     \   /
      v v
       S
      / \
     v   v
     W   G
    ```
    \(P(E, B, S, W, G) = P(B)P(E)P(S|EB)P(W|S)P(G|S)\)
    We thus know this CPT

    | |g|-g|
    |-|-|--|
    |s|0.5|0.5|
    |-s|0|1|

    
2. We know that \(S\) is true as evidence (\(S = s\)). Then, what is the probability of \(G = True\), that is \(P(g|s)\) = 0.5

3. If \(G\) is true, what is the probability \(P(S = s|g)\)? 

    By Bayes Law, we have 

    \[
        P(S|g) = \frac{P(g|S)P(S)}{P(g)}
    \]

    And we know the probability of \(P(g|S)\)
    We also know \(P(-s|g) + P(s | g) = 1\)

    \[
        P(-s|g) = \frac{P(g|-s)P(s)}{P(-g)} = 0
    \]

    (by table)

    Hence \(P(s|g) = 1\).

    We could have figured this out by the CPT. We have \(-s \implies -g\). Then contrapositive \(g \implies s\). Hence \(P(s | g) = 1\). We can use this when the probablities are 0 and 1.

4. What is \(P(G | S, W)\)?
   This is a table of 8 values
   \(P(g | s, w)\) \(P(g | s, -w)\).  

   However we can take advantage of d-separation. Given \(S\), \(G\) and \(W\) are independent, so \(P(g | s, w) = P(g|s, -w) = P(g | s) = 0.5\) (by CPT).

5. What about \(P(G|W)\)
   This is a table of 4 values, but we don't know any evidence so we need to use variable elimination.

   We need 2 runs where \(W = w\) and \(W = -w\).

   |  |g|-g|
   |--|-|--|
   |w | |  |
   |-w| |  |

   The VE run will give us \(P(G|w)\) and \(P(G|-w)\) and will give us values for both \(G=g\) and \(G=-g\).

   Everything in this network is relevant, since our query variable is \(G\). If we eliminate \(E\) and \(B\) before \(S\),
   we will 

   So we choose this ordering of buckets.
   Note that each bucket must have all the CPTs that mention the variable

   | |1|2|3|4|
   |-|-|-|-|-|
   |E|\(P(E)P(S, E B)\)| - |
   |B|\(P(B)\)|\(P(B)F_1(S, B)\)|
   |S|\(P(w \| S)P(G\|S)\)| - |\(P(w\|S) P(G\|S) F_2(S)\)|
   |G|-|-|-|\(F_3(G)\)|

   Summing out \(E\), we get a factor \(F_1(S, B)\)
   \(F_1(s, b) = P(e)P(s|e,b) + P(-e)P(s|-e, b) = 0.1 * 0.9 + 0.9 * 0.8 = 0.81\)
   \(F_1(-s, b) = 0.19\)
   \(F_1(s, -b) = 0.02\)
   \(F_1(-s, -b) = P(e)P(-s|-b,e) + P(-e)P(-s|-b, -e) = 0.1 * 0.8  + 0.9 * 1.0 = 0.91\)

   Summing out \(B\), we get a factor \(F_2(S)\)
   \(F_2(s) = 0.901\)
   \(F_2(-s) = 0.099\)

   Summing out \(S\) we get
   \(F_3(g) = 0.0396\)
   \(F_3(-g) = 0.2198\)

   Then \(P(G|w) =  normalize(F_2(G))\)
   And we get
   \(P(-g | W) = 0.8473\) and \(P(g | W) = 0.1527\)

   
   | |1|2|3|4|
   |-|-|-|-|-|
   |E|\(P(E)P(S, E B)\)| - |
   |B|\(P(B)\)|\(P(B)F_1(S, B)\)|
   |S|\(P(-w \| S)P(G\|S)\)| - |\(P(-w\|S) P(G\|S) F_2(S)\)|
   |G|-|-|-|\(F_3(G)\)|

   Then we get \(P(-g | -w) = 0.9866\) \(P(g | -w) = 0.0135\)

 