---
tags: 
  - correctness
  - recursive
  - iterative
---

# 2018-10-25 Recursive and iterative correctness

Postconditions of the recursive calls are going to produce a good claim for termination.

> **Precondition**: \(A\) is sorted, comparable with \(x\).
> **Postcondition**: \(0 \leq p \leq n\) and \(A[0...p-1] < x \leq A[p...n-1]\) (x is between p-1 and p). 

```python
  while b <= e:
    m = (b+e) // 2
    if A[m] < x: # ..., A[m-1],  A[m] < x [b can be here] < 
      b = m + 1 # area leq should be behind b
    else: # A[m] >= x
      e = m - 1 # area geq should be just past e
    return b
```

If the precondition is fulfilled and the program runs, does it work?

**Preconditions**
- \(A\) sorted non-decreasing and elements are comparable with \(x\) `len(A)` = \(n > 1\). `b = 0`, `e = n-1`


**Postconditions**

- \(0 \leq b \leq n\) to ensure that \(b\) doesn't overflow.
- \(\forall j \in A[0:b], j < x\)
- \(\forall k \in A[b:n], k \geq x\)
    - since we shift \(b\) to have values \(A[b] < x\).

**Loop Invariants**
Want things that resemble the postcondition
- \(P(i): \) At the end of the \(i\)th iteration (if it occurs), \(0 \leq b_i \leq e_i + 1 \leq n\). \(b_i\) never gets  \(e_i + 1\), where \(X_i\) is the value of \(X\) after the loop iterates \(i\) times.
We want a loop invariant that is true at the last loop, to show termination
    - \(b_i, e_i \in \mathbb{N}\)
    - \(\forall j \in A[0:b].  j < x \land \forall k \in A[e+1:n].  k \geq x\)

Want to prove \(\forall i \in \mathbb{N}. P(i)\) using simple induction.

> Let \(i \in \mathbb{N}\), assume \(P(i)\).
> **Case \(i = 0\):**
>   The loop hasn't done anything, so by precondition, \(0 = b_0 \leq n - 1 = e_0\) Also \(0, n-1 \in \mathbb{N}\). Both slices are empty, any universally quantified statement is vacuously true.
> **Inductive Step**
> Let \(i \in \mathbb{N}\). Assume \(P(i)\). If there is an \(i + 1\)th iteration of the loop, then \(b_i \leq e_i\), because if the equality is not true, then the loop would terminate. Thus let by code, \(m = ((b_i + e_i) //  2) \in \mathbb{N}\). Notice that \(2b_i // 2 \leq m \leq 2e_i // 2\)
> 
> **Case \(A[m] < x\)**
> \(b_{i + 1} = m+1\), and \(e_{i + 1} = e_{i}\)
> By the IH, \(P(i) \implies e_{i+1} = e_i\), so \(A[e_{i+1}:n] = A[e_{i}:n]; \forall j \in A[e_{i+1}:n] j \leq x\) 
> Since \(m \leq e_{i+1}, 0 \leq b_{i+1} = m + 1 \leq e_i + 1 = e_{i+1} + 1 \leq n\)
> \(A[m] < x \), so \(\forall k \in A[0:m+1], k < x\), but \(b_{i+1} = m + 1\)
> Notice also that since \(e_{i+1} = e_i\land. b_{i + 1} = m + 1 \in \mathbb{N}\)
> Since all post-conditions are still true, \(P(i+1)\) follows.
>
> **Case \(A[m] \geq x\)**
> In this case, \(e_{i+1} = m - 1\), and \(b_{i+1} = b_i\)
> By IH, \(\forall j \in A[0:b_i].  j < x\). But \(b_i= b_{i+1}\), so \(\forall j \in A[0:b_{i+1}]. j < x\)
>
> Also since \(A[m] = A[e_{i+1} + 1] \geq x\), we know that \(\forall k \in A[e_{i+1}:n], k \geq x\). Also we know \(0 \leq b_i = b_{i+1} \leq m = e_{i+1} + 1 \leq e_i + 1 < n\) by IH
> Also by IH, \(b_i, e_i \in \mathbb{N}\), so \(b_{i+1} = b_i \in \mathbb{N}\), and \(e_{i + 1} = m - 1 \in \mathbb{N} \geq b_1 \geq 0\).


We have now partial correctness. For total correctness, we need to show that the preconditions imply termination.

> Assume preconditions satisfied, and code executes and terminates. Call the last iteration of loop \(f\). By the loop conditions, terminates when \(b_f > e_f\). By the loop invariant, \(b_f  \leq e_f + 1\). Since they are integers, must have \(b_f = e_f + 1\). Thus by loop invariant, we have \(\forall j \in A[0:b_f]. j < x\) and \(\forall k \in A[b_f:n], k \geq x\).
> 
> Define \(a_i = e_i + 1 - b_i\). Show that \(a_i\) is decreasing sequence of naturals.
By loop invariant, \(e_i + 1 \geq b_i\) and \(e_i, b_i \in \mathbb{Z}\), so \(e_i + 1 - b_i \in \mathbb{N}\).
> 
> Suppose there is an \(i + 1\)th iteration.
>
> **Case \(e_{i+1} = e_i\) and \(b_{i+1} = m + 1\)**
> We know \(e_i = e_{i + 1} \geq m\), so \(e_i = e_{i+1} + 1 - b_i = e_{i} + 1 - m - 1 = e_i - m < e _{i} + 1 - b_i\) because \(m \geq b_i\)
> 
> **Case \(e_{i+1} = m-1\) and \(b_{i+1} = b_i\)**
> Can show \(e_{i+1} + 1 - b_{i+1} < e_{i} + 1 - b_i\)
>
> Thus \(a_i\) is a decreasing sequence in \(\mathbb{N}\).