---
tags:
 - "recurrences"
---
# 2018-09-27 

Define 

\[
f(n) =
\begin{cases}
2 & n=0\\
7 &n=1\\
2f(n-2)+f(n-1)&n>1
\end{cases}
\]

We conjecture that 

\[
\forall n \in \mathbb{N} ,f(n) < 2^{n+2}
\]

Let \(n\) be an arbitrary natural number. Assume \(P(0)...P(n-1)\). 

Case \(n \geq 2\).

Since \(n \geq 2\), \(f(n) = 2f(n-2) + f(n-1)\), which is **less than** \(2 \cdot 2^n + 2^{n+1} = 2^{n+2}\)
... case n = 1, case n =0 trivial.


## Fibbonaci

Define the \(n\)th Fibonacci number as follows

\[
F(n) = \begin{cases} n&n<2 \\ F(n-2) + F(n-1) & n\geq 2\end{cases}
\]

Note some basic cases

|\(n\)|\(F(n)\)|Sum|
|----|--------|----|
|0|0|0|
|1|1|1|
|2|1|2|
|3|2|4|
|4|3|7|
|5|5|12|
|6|8|20|
|7|13|33|
|8|21|54|
|9|32|..|
|10|55|...|


Notice that the sum of the fibonacci sequence resembles the fibonacci sequence. Can we prove that \(P(n) := \sum_{i=0}^{i=n} F(i) = F(n+2)-1\)?

**Proof**
Let \(n \in \mathbb{N}\). 

Base case: \(\sum_{i=0}^{i=n}F(i) = F(0) = 0 = F(2) - 1 = 1-1\)
Base case: \(F(0) + F(1) = 0 + 1 = 1 = F(3) - 1 = 2-1\)
case \(n \geq 1\). Then \(F(0) + ... +F(n) + F(n+1) = F(n+2) - 1 + F(n+1)\) by the inductive hypothesis \(P(n)\).
Then by definition of \(F\), we write \(F(n+2) + F(n+1) = F(n+3)\) (since \(n+3 \geq 2\)), hence we have the sum equal to \(F(n+3) -1\), which completes the proof.

Which fibonacci number is a multiple of 5? Notice that every 5 numbers seem to be multiple of 5. How can we prove \(P(n) := 5 | F(5n)\)?

Base case: \(F(5 \cdot 0) = 0 = 5 \cdot 0\).
Inductive step: Let \(n \in \mathbb{N}\). Assume \(P(n)\), that is that \(5 | F(5n)\), and such let \(k \in \mathbb{N}. F(5n) = 5k\).

Then 

\[
F(5n + 5) = F(5n + 3) + F(5n+4) 
\]
\[
= F(5n+2)+F(5n+1) + F(5n+3) + F(5n+2)
\]
\[
= 2(F(5n) + F(5n+1)) + F(5n+1) + F(5n+2) + F(5n+1)
\]
\[
= 3(F(5n) + F(5n+1)) + 2F(5n+1)
\]
\[
=3(5k) + 5F(5n+1)
\]

## Recurrances

The fibonacci sequence has a closed form expression.

\[
F(n) = \frac{\phi^n - \Phi^n}{\sqrt{5}}
\]

Where 

\[
\phi = \frac{1+\sqrt{5}}{2}, \Phi = \frac{1-\sqrt{5}}{2}
\]

We also have the relation for the Fib. sequence

\[
r^n = r^{n-1} + r^{n-2} \implies r^2 = r+1
\]

The two solutions to this equation is when \(\phi = r_1\), and \(\Phi = r_2\)