# 2019-11-15

State operations

```haskell
get :: State s s
get = State (\state -> (state, state))

put :: s -> State s ()
put x = State (\_ -> ((), x))
```

`()` is the unit value.


```haskell
runState :: State s a -> (s -> (a, s))
runState (State f) = f
-- or equivalently
runState :: State s a -> s -> (a, s)
runState (State f) init = f init
```

> The Haskell type State describes functions that consume a state and produce both a result and an updated state, which are given back in a tuple.

Then our `fibCounted` can be written

```haskell
-- the first argument to State is the state type
-- the second is the produced value, the fib number
fibCounted :: Integer -> State Integer Integer
fibCounted 0 = State $ \count -> (0, count + 1)
fibCounted 1 = State $ \count -> (1, count + 1) -- return new value, and new state 
fibCounted n = State $ \count0 ->
    let (f1, count1) = runState (fibCountedS (n-1)) count0
        (f2, count2) = runState (fibCountedS (n-2) count1
        (f3, count3) = runState (State $ \c -> (f1 + f2, c + 1)) count2
    in 
        (f3, count3)
```

How can we 'chain' this? We've increased the amount of boilerplate code!

Consider `andThen`

```haskell
andThen :: State s a -> State s b -> State s b
andThen stateOp1 stateOp2 = State $ \state0 ->
    let (x1, s1) = runState stateOp1 state0
        (x2, s2) = runState stateOp2 s1
    in 
        (x2, s2)

fibCounted n = (fibCounted (n - 1)) `andThen`
    (fibCounted (n - 2)) `andThen`
    (State $ \c -> (f1 + f2, c + 1))
```

Note that the `x1` in andThen is never used! `f1` and `f2` are not in scope!


```haskell
bind :: State s a -> (a -> State s b) -> State s b
bind stateOp1 stateOpMaker2 = State $ \state0 ->
    let (x1, state1) = runState stateOp1 state0
        (x2, state2) = runState (stateOpMaker2 x1) state1
    in 
        (x2, state2)

fibCounted n = (fibCounted (n - 1)) `bind` (\f1 ->
                    (fibCounted (n - 2)) `bind` (\f2 ->
                         (State $ \c -> (f1 + f2, c + 1))))
```

This will run the state operation, take the result, and pass it to the next function.


Can we generalize `bind :: State s a -> (a -> State s b) -> State s b`

oh boy here it comes

```haskell
class Monad m where
    (>>=) :: m a -> (a -> m b) -> m b
```

Consider this as doing something with `m a`, then use the value in another computation, producing an `m b`.

Then we can write

```haskell
fibCounted n = (fibCounted (n - 1)) >>= \f1 ->
               (fibCounted (n - 2)) >>= \f2 ->
               (state $ \c -> (f1 + f2, c + 1))
```
With `do` notation

```haskell
fibCounted n = 
    do
        f1 <- fibCounted (n - 1)
        f2 <- fibCounted (n - 2)
        state $ \c -> (f1 + f2, c + 1)
```