# 2017-02-05.1

## Proof by Induction

Induction is to prove a statement \(P\) for a natural number 0. Then we assume \(P\) holds for an arbitrary natural number \(k\), and then prove the statement for \(k + 1\). Induction can be applied to anything that can be framed as an ordered set.

> *Example*
> **Theorem.** \(\forall n \in \mathbb{N} \sum_{i=1}^n i = \frac{n(n+1)}{2}\)
> **Proof.** Let \(P(n):\sum_{i=1}^n i = \frac{n(n+1)}{2}\).
> *Base Case*. \(P(0) : \sum_{i=1}^0 i = 0\)
> *Inductive Step*.  Let \(k \in \mathbb{N}\) Assume \(P(k)\). We want to show \(P(k) \Rightarrow P(k+1)\). \(P(k)\) implies that  \(\sum_{i=1}^k i = \frac{k(k+1)}{2}\). Then we have \(\sum_{i=1}^{k+1} i = \sum_{i=1}^{k} i + (k+1) =  \frac{k(k+1)}{2} + (k+1)\) by the induction hypothesis.
> \(\frac{k(k+1)}{2} + (k+1) = \frac{k(k+1) + 2(k+1)}{2} = \frac{(k+1)(k+2)}{2}\).
> \(\blacksquare\)

In general we are proving for a proposition \(P\),

\(P(0) \land \forall k \in \mathbb{N} P(k) \Rightarrow P(k+1)\).