# 2018-01-24

We generalize the previous example to generalize for all \(d \in \mathbb{Z}\).

> **Theorem**. \(\forall x, d \in \mathbb{Z}. Divides(x, x+d) \Rightarrow Divides(x, d)\).
> *Proof* Let \(x, d \in \mathbb{Z}\). By the definition of \(Divides\), \(\exists k \in \mathbb{Z}\) such that \(xk = x + d\). Hence let \(k\) be as such. We want to show \(\exists k' \in \mathbb{Z}. xk' = d\). Take \(k' = (k - 1)\). Then we have \(xk' = x(k-1) = xk - x = d\) since \(xk = x+d \Rightarrow xk-x = d\) 
> \(\blacksquare\)

The proof is a series of true statements where each statements follows logically from
  1. Definitions 
  2. Assumptions (stuff in header)
  3. Previous statements
  4. External claims that have previously been proven.

We will give an example of using external claims. Remember the following definition of a prime number.

> **Definition.** \(Prime(n) : (n > 1 ) \land \forall x \in \mathbb{N}. (x \neq 1 \land x \neq n) \Rightarrow \lnot Divides(x, n)\)

Then we will attempt to prove the following theorem using the previous proof for \(Divides\).

> **Theorem.** \(\forall x, d \in \mathbb{N}, Prime(d) \land Divides(x, x+d) \Rightarrow (x=1 \lor x = d))\)
> *Proof.* Let \(d \in \mathbb{N}\) be a prime number.  Let \(x \in \mathbb{N}\) be such that \(Divides(x, x+d).\)
> From the previous theorem, we know \(Divides(x, x+d) \Rightarrow Divides(x, d)\), since \(\mathbb{N} \subset \mathbb{Z}\).
> Hence from the definition of \(Prime\), we take the contrapositive \(Prime(p): \forall z \in \mathbb{N}, Divides(z, p) \Rightarrow (z = 1 \lor z = p)\). Hence by the definition of prime we have that since \(d\) is prime, we must have \(x = 1 \lor x = d\).
> \(\blacksquare\)