# 2018-02-07
> *Example*
> Prove \(\forall x, y \in \mathbb{Z}, \forall n \in \mathbb{N}, 5 | (x-y) \Rightarrow 5|(x^n - y^n)\).
> Notice that we are quantifying over multiple "variables" this time rather than induction on one variable.
> **Proof.** Let \(x, y \in \mathbb{Z}\). We want to prove \(P(n) := \forall n \in \mathbb{N}. (5 | (x-y) \Rightarrow 5 | (x^n - y^n)\).
> *We have fixed \(x, y\), so now \(n\) is the only variable. For this course, we usually have only one free variable to manipulate.
> *Base Case.* \(P(0): 5 | x-y \Rightarrow 5 | (x^0 - y^0)\).
> \(x^0 - y^0 = 0\). Hence \(5 | 0\).
> *Inductive Step.** Let \(k \in \mathbb{N}\), and assume \(P(k)\). We want to show \(P(k+1) : 5 (x-y) \Rightarrow 5 | (x^{k+1} - y^{k+1})\).
> 
> \(P(k) \equiv 5 | (x-y) \Rightarrow 5 | (x^k - y^k).\) 
> Let \(c \in \mathbb{Z}\) be such that \(5c = (x-y)\). Since we have assumed \(P(k)\) and assumied \(5 | x-y\), we also know \(5 | (x^k-y^k)\). Then let \(q \in \mathbb{Z}\) be such that \(5q = (x^k - y^k)\). Then \(5qy = y(x^k-y^k) = (yx^k - y^{k+1})\), and \(5cx^k = x^k(x-y) = x^{k+1} - yx^k\)
. We have then \(5cx^k + 5qy = (x^{k+1} - yx^k + yx^k - y^{k+1}) = (x^{k+1} - y^{k+1}) = 5(cx^k + qy)\)
> Let \(u = (cx^k + qy)\), then \(5u =  (x^{k+1} - y^{k+1})\).
> Therefore 5 divides \(x^{k+1} - y^{k+1}\). By induction, \(\forall n \in \mathbb{N}, 5 | x- y \Rightarrow 5 | x^n - y^n\)
> Therefore \(\forall x, y \in \mathbb{Z}, \forall n \in \mathbb{N}, 5 | (x-y) \Rightarrow 5|(x^n - y^n)\)
> \(\blacksquare\)
> 
There is a second way to prove this where we do not fix \(x\) and \(y\). Since all variables are universally quantified, we can say \(\forall n \in \mathbb{N}, \forall x, y \in \mathbb{Z}, 5 | (x-y) \Rightarrow 5|(x^n - y^n)\). 

> Let \(P(n): = \forall x, y \in \mathbb{Z}, 5 | (x-y) \Rightarrow 5|(x^n - y^n)\). We are proving by induction on \(n\), that \(P(n)\) is true for every \(x, y\).

> \(P(0) \equiv \forall x, y \in \mathbb{Z}. 5|x-y \Rightarrow 5 | x^0 - y^0\)
> Let \(x, y, \in \mathbb{Z}\). Let \(k = 0\), then \(5k = 0\), so \(5 | x^0 - y^0\).
> Let \(k \in \mathbb{N}\). Assume \(P(k)\). Fix \(x, y\), proof procedes as above. Notice that we are fixing \(x, y\) separately than above.