# 2018-01-29.0

## Proof by Cases
> *Example*
> We define \(Even(x)\) to be a predicate \(\mathbb{N} \rightarrow \mathbb{N}\) such that \(Even(x) := \exists n \in \mathbb{N} x=2n\).
> **Theorem**
> \(\forall x, y \in \mathbb{N}, Even(x) \lor Even(y) \lor Even(x+y)\)
> *Proof*
> Let \(x, y \in \mathbb{N}\).
> **Case 1** \(Even(x)\). Then the statement is true.
> **Case 2** Similarly for Case 1, \(Even(y)\).
> **Case 3** \(\lnot Even(x) \land \lnot Even(y)\).
> Then, \(\exists k \in \mathbb{N}, 2k + 1 = x\) and \(\exists k \in \mathbb{N}, 2k + 1 = y\), because x and y are odd. Let \(k_1\), \(k_2\) be such that \(2k_1 +1 = x\) and similarly with \(y\) for \(k_2\). Then let \(k = k_1 + k_2 + 1\). Then \(x + y = 2 k_1 + 2k_2 + 2 = 2(k_1+k_2+1) = 2k\). \(\blacksquare\)

> *Example*
> **Definition**
> \(\forall d, N \in \mathbb{N}, d | N \Leftrightarrow \exists k \in \mathbb{Z}, N = dk\).
> \(\forall p \in \mathbb{N}, Prime(p) \Leftrightarrow  p > 1 \land . \forall d \in \mathbb{N}, d | p \Rightarrow d = 1 \lor d = p\)
> **Theorem**
> \(\forall d \in \mathbb{N}. \forall a, b, \in \mathbb{N}, d \lnot | a \land d \lnot | b \Rightarrow d \neg | ab \Leftrightarrow d \leq 1 \lor Prime(d)\)

> **Proof**
> Since the statement is biconditional, we must prove two things, that 
>  1. \(\forall d \in \mathbb{N}. \forall a, b \in \mathbb{N} d \neg | a \land d \neg | b \Rightarrow Prime(d) \lor d \leq 1\)
>  Contrapositively, \(\forall d \in \mathbb{N}. \lnot Prime(d) \land d > 1 \Rightarrow \exists a, b, \in \mathbb{N}. d \neg a \land d \neg b \land d | ab\)
 > 2. \(\forall d \in \mathbb{N}. Prime(d) \lor \leq 1 \Rightarrow \forall a, b, \in \mathbb{N}. d \neg | a \land d \neg b \Rightarrow d \neg ab\)

> Let \(d \in \mathbb{N}\) such that \(d\) is not Prime, and \(d > 1\). By definition of Prime, either \(d \leq 1\), or \(\exists k \in \mathbb{N}, k | d \land k \neq 1 \land n \neq d\), we have a number \(k\) such that \(kc = d\) by the definition of \(Divides\). We want to show \(d \neg | k \land d \neg | c\). 